src/PermCacheDef.v
@@ -1,0 +1,134 @@
+Require Import List.
+Require Import FMapAVL.
+Require Import FMapFacts.
+Require Import Word.
+Require Import Array.
+Require Import Mem Pred.
+Require Import WordAuto.
+Require Import Omega.
+Require Import AsyncDisk.
+Require Import ListUtils.
+Require Import OrderedTypeEx.
+Require Import PeanoNat Nat Arith.
+Require Import MapUtils.
+Require Import MemPred.
+Require Import ListPred.
+Require Import FunctionalExtensionality.
+Require Export PermProgMonad PermSec.
+Require Export PermHoare PermSepAuto.
+Require Export PermSecInstr.
+Require Import ADestructPair DestructVarname.
+
+Import AddrMap.
+Import Map MapFacts.
+Import ListNotations.
+
+Set Implicit Arguments.
+
+Definition eviction_state : Type := unit.
+Definition eviction_init : eviction_state := tt.
+Definition eviction_update (s : eviction_state) (a : addr) := s.
+Definition eviction_choose (s : eviction_state) : (addr * eviction_state) := (0, s).
+
+Definition h_cachemap := t (handle * bool).
+
+Record h_cachestate :=
+  mk_cs {
+      HCSMap : h_cachemap;
+      HCSMaxCount : nat;
+      HCSCount : nat;
+      HCSEvict : eviction_state
+    }.
+
+Definition cache0 sz := mk_cs (Map.empty _) sz 0 eviction_init.
+
+
+ (** rep invariant *)
+
+Definition size_valid cs :=
+  cardinal (HCSMap cs) = HCSCount cs /\
+  cardinal (HCSMap cs) <= HCSMaxCount cs /\
+  HCSMaxCount cs <> 0.
+
+Definition addr_valid (d: tagged_disk) (cm : h_cachemap) :=
+  forall a, In a cm -> d a <> None.
+
+Definition addr_clean (cm : h_cachemap) a :=
+    find a cm = None \/ exists v, find a cm = Some (v, false).
+
+Definition addrs_clean cm al :=
+  Forall (addr_clean cm) al.
+
+Definition cachepred (cache : h_cachemap) (bm: block_mem) (a : addr) (tb: tagged_block ): @Pred.pred _ addr_eq_dec tagged_block :=
+  (match find a cache with
+   | None => a |-> tb
+   | Some (h, false) => a |-> tb * [[ bm h = Some tb ]]
+   | Some (h, true)  => exists tb0, a |-> tb0 * [[ bm h = Some tb ]]
+   end)%pred.
+
+Definition rep (cs : h_cachestate) (m : tagged_disk) (bm: block_mem): @Pred.pred _ addr_eq_dec tagged_block :=
+  ([[ size_valid cs /\
+      addr_valid m (HCSMap cs) ]] *
+   mem_pred (HighAEQ:= addr_eq_dec) (cachepred (HCSMap cs) bm) m)%pred.
+
+Definition h_writeback a (cs : h_cachestate) :=
+  match find a (HCSMap cs) with
+  | Some (h, true) =>
+      Bind (Write a h)
+           (fun _ => Ret (mk_cs (Map.add a (h, false) (HCSMap cs))
+                             (HCSMaxCount cs) (HCSCount cs)
+                             (HCSEvict cs)))
+  | _ =>
+    Ret cs
+  end.
+
+Definition h_evict' a cs:=
+  match find a (HCSMap cs) with
+  | Some _ =>
+    Ret (mk_cs (Map.remove a (HCSMap cs))
+               (HCSMaxCount cs) (HCSCount cs - 1) (HCSEvict cs))
+  | None =>
+    Ret (mk_cs (Map.remove a (HCSMap cs))
+               (HCSMaxCount cs) (HCSCount cs) (HCSEvict cs))
+  end.
+
+Definition h_evict a cs:=
+  Bind (h_writeback a cs)
+       (fun cs => h_evict' a cs).
+
+Definition h_maybe_evict (cs : h_cachestate) : prog h_cachestate :=
+  if (lt_dec (HCSCount cs) (HCSMaxCount cs)) then
+    Ret cs
+  else 
+    let (victim, evictor) := eviction_choose (HCSEvict cs) in
+    match find victim (HCSMap cs) with
+    | Some _ =>
+      h_evict victim (mk_cs (HCSMap cs)
+          (HCSMaxCount cs) (HCSCount cs) evictor)
+    | None => (* evictor failed, evict first block *)
+      match (Map.elements (HCSMap cs)) with
+      | nil => Ret cs
+      | (a, v) :: tl => h_evict a cs
+      end
+    end.
+
+Definition h_read a cs :=
+    cs <- h_maybe_evict cs;;
+    match Map.find a (HCSMap cs) with
+    | Some (h, dirty) => Ret (cs, h)
+    | None =>
+      h <- Read a;;
+      Ret (mk_cs (Map.add a (h, false) (HCSMap cs))
+                 (HCSMaxCount cs) (HCSCount cs + 1) (eviction_update (HCSEvict cs) a), h)
+    end.
+
+Definition h_write a h cs:=
+    cs <- h_maybe_evict cs;;
+    match Map.find a (HCSMap cs) with
+    | Some _ =>
+      Ret (mk_cs (Map.add a (h, true) (HCSMap cs))
+                 (HCSMaxCount cs) (HCSCount cs) (eviction_update (HCSEvict cs) a))
+    | None =>
+      Ret (mk_cs (Map.add a (h, true) (HCSMap cs))
+                 (HCSMaxCount cs) (HCSCount cs + 1) (eviction_update (HCSEvict cs) a))
+    end.
