src/PermCacheLemmas.v
@@ -1,0 +1,253 @@
+Require Import List.
+Require Import FMapAVL.
+Require Import FMapFacts.
+Require Import Word.
+Require Import Array.
+Require Import Pred.
+Require Import WordAuto.
+Require Import Omega.
+Require Import AsyncDisk.
+Require Import ListUtils.
+Require Import OrderedTypeEx.
+Require Import Arith.
+Require Import MapUtils.
+Require Import MemPred.
+Require Import ListPred.
+Require Import FunctionalExtensionality.
+Require Export PermCacheDef.
+Require Import ADestructPair DestructVarname.
+
+Import AddrMap.
+Import Map.
+Import ListNotations.
+
+Set Implicit Arguments.
+
+Lemma find_elements_hd:
+  forall T a (v:T) l m,
+    elements m = (a, v)::l ->
+    find a m = Some v.
+Proof.
+  intros.
+  apply find_1.
+  assert (A: InA (fun a b =>  fst a = fst b /\ snd a = snd b)
+                 (a,v) (elements m)).
+  rewrite H; apply InA_cons_hd; auto.
+  apply elements_2 in A; auto.
+Qed.
+
+
+
+  Lemma cachepred_remove_invariant : forall a a' v cache bm,
+    a <> a' -> cachepred cache bm a v =p=> cachepred (Map.remove a' cache) bm a v.
+  Proof.
+    unfold cachepred; intros.
+    rewrite MapFacts.remove_neq_o; auto.
+  Qed.
+
+  Lemma cachepred_add_invariant : forall a a' v v' cache bm,
+    a <> a' -> cachepred cache bm a v =p=> cachepred (Map.add a' v' cache) bm a v.
+  Proof.
+    unfold cachepred; intros.
+    rewrite MapFacts.add_neq_o; auto.
+  Qed.
+
+Lemma mem_pred_cachepred_remove_absorb : forall csmap d a w bm,
+    d a = Some w ->
+    mem_pred (HighAEQ:= addr_eq_dec) (cachepred csmap bm) (mem_except d a) * a |-> w =p=>
+    mem_pred (HighAEQ:= addr_eq_dec) (cachepred (remove a csmap) bm) d.
+  Proof.
+    intros.
+    eapply pimpl_trans; [ | apply mem_pred_absorb_nop; eauto ].
+    unfold cachepred at 3.
+    rewrite MapFacts.remove_eq_o by auto.
+    cancel; eauto.
+    rewrite mem_pred_pimpl_except; eauto.
+    intros; apply cachepred_remove_invariant; eauto.
+  Qed.
+
+
+Lemma addr_clean_cachepred_remove_none :
+  forall cs a d bm,
+    find a (HCSMap cs) = None ->
+    mem_pred (HighAEQ:= addr_eq_dec) (cachepred (HCSMap cs) bm) d =p=>
+      mem_pred (HighAEQ:= addr_eq_dec) (cachepred (remove a (HCSMap cs)) bm) d.
+Proof.
+  intros.
+  eapply mem_pred_pimpl; intros.
+  destruct (Nat.eq_dec a a0); subst.
+  unfold cachepred; simpl; cleanup.
+  rewrite MapFacts.remove_eq_o; auto.
+  eapply cachepred_remove_invariant; eauto.
+Qed.  
+
+Lemma addr_clean_cachepred_remove :
+  forall cs a d F vs bm,
+    addr_clean (HCSMap cs) a ->
+    (F * a |-> vs)%pred d ->
+    mem_pred (HighAEQ:= addr_eq_dec) (cachepred (HCSMap cs) bm) d =p=>
+      mem_pred (HighAEQ:= addr_eq_dec) (cachepred (remove a (HCSMap cs)) bm) d.
+  Proof.
+    unfold addr_clean; intros.
+    apply ptsto_valid' in H0; cleanup.
+    destruct H; cleanup.
+    - rewrite mem_pred_extract with (a := a) by eauto.
+      unfold cachepred at 2; rewrite H.
+      cancel.
+      rewrite sep_star_comm.
+      eapply mem_pred_cachepred_remove_absorb; eauto.
+    - rewrite mem_pred_extract with (a := a) by eauto.
+      unfold cachepred at 2; rewrite H.
+      rewrite sep_star_comm.
+      cancel.
+      eapply mem_pred_cachepred_remove_absorb; eauto.
+  Qed.
+
+  Lemma addr_valid_ptsto_exists:
+      forall a b cs d,
+        addr_valid d (HCSMap cs) ->
+        find a (HCSMap cs) = Some b ->
+        exists F tb, (sep_star (AEQ:=addr_eq_dec) F (a|->tb))%pred d.
+    Proof.
+      unfold rep, addr_valid; intros.
+      destruct_lift H.
+      assert (A: find a (HCSMap cs) <> None ).
+      intuition; congruence.
+      apply MapFacts.in_find_iff in A.
+      specialize (H _ A).
+      destruct (d a) eqn:D; try congruence.
+      do 2 eexists.
+      apply any_sep_star_ptsto; eauto.
+    Qed.
+
+  Lemma size_valid_remove : forall cs a,
+    size_valid cs ->
+    Map.In a (HCSMap cs) ->
+    size_valid (mk_cs (Map.remove a (HCSMap cs)) (HCSMaxCount cs) (HCSCount cs - 1) (HCSEvict cs)).
+  Proof.
+    unfold size_valid in *; intuition simpl.
+    rewrite map_remove_cardinal by eauto; congruence.
+    eapply le_trans.
+    apply map_cardinal_remove_le; auto.
+    auto.
+  Qed.
+
+  Lemma size_valid_remove_notin : forall cs a,
+    size_valid cs ->
+    ~ Map.In a (HCSMap cs) ->
+    size_valid (mk_cs (Map.remove a (HCSMap cs)) (HCSMaxCount cs) (HCSCount cs) (HCSEvict cs)).
+  Proof.
+    unfold size_valid in *; intuition simpl.
+    rewrite Map.cardinal_1 in *.
+    rewrite map_remove_not_in_elements_eq by auto. auto.
+    eapply le_trans.
+    apply map_cardinal_remove_le; auto.
+    auto.
+  Qed.
+
+  Lemma size_valid_remove_cardinal_ok : forall cs a,
+    size_valid cs ->
+    Map.In a (HCSMap cs) ->
+    Map.cardinal (Map.remove a (HCSMap cs)) < HCSMaxCount cs.
+  Proof.
+    unfold size_valid; intros.
+    rewrite map_remove_cardinal.
+    omega.
+    apply In_MapsTo; auto.
+  Qed.
+
+  Lemma size_valid_cache0 : forall cachesize,
+    cachesize <> 0 ->
+    size_valid (cache0 cachesize).
+  Proof.
+    unfold size_valid, cache0; simpl; intros.
+    rewrite Map.cardinal_1.
+    rewrite MapProperties.elements_empty.
+    intuition.
+  Qed.
+
+  Lemma addr_valid_remove : forall d a cm,
+    addr_valid d cm ->
+    addr_valid d (Map.remove a cm).
+  Proof.
+    unfold addr_valid; intros.
+    apply H.
+    eapply MapFacts.remove_in_iff; eauto.
+  Qed.
+
+  Lemma addr_valid_empty : forall m,
+    addr_valid m (Map.empty (handle * bool)).
+  Proof.
+    unfold addr_valid; intros.
+    apply MapFacts.empty_in_iff in H.
+    exfalso; auto.
+  Qed.
+
+  Lemma addr_valid_mem_valid : forall a cm c d,
+    Map.find a cm = Some c ->
+    addr_valid d cm ->
+    exists vs, d a = Some vs.
+  Proof.
+    intros.
+    assert (Map.In a cm).
+    apply MapFacts.in_find_iff.
+    destruct (Map.find a cm); try congruence.
+    specialize (H0 _ H1).
+    destruct (d a); try congruence; eauto.
+  Qed.
+
+  Lemma size_valid_add :
+    forall cs evictor vv a,
+    cardinal (HCSMap cs) < HCSMaxCount cs ->
+    Map.find a (HCSMap cs) = None ->
+    size_valid cs ->
+    size_valid (mk_cs (add a vv (HCSMap cs)) (HCSMaxCount cs) (HCSCount cs + 1) evictor).
+  Proof.
+    unfold size_valid; intuition; simpl.
+
+    destruct (find a0 (HCSMap cs)) eqn:?; try congruence.
+    rewrite map_add_cardinal. omega.
+    intuition repeat deex.
+    apply MapFacts.find_mapsto_iff in H3; congruence.
+
+    destruct (Map.find a0 (HCSMap cs)) eqn:?.
+    rewrite map_add_dup_cardinal; auto.
+    eexists; eapply MapFacts.find_mapsto_iff; eauto.
+    rewrite map_add_cardinal. omega.
+    intuition repeat deex.
+    apply MapFacts.find_mapsto_iff in H3; congruence.
+  Qed.
+
+  Lemma addr_valid_add : forall d cm a vv v,
+    d a = Some v ->
+    addr_valid d cm ->
+    addr_valid d (Map.add a vv cm).
+  Proof.
+    unfold addr_valid; intros.
+    destruct (addr_eq_dec a a0); subst; try congruence.
+    apply H0.
+    eapply MapFacts.add_in_iff in H1; intuition.
+  Qed.
+
+  
+  Lemma mem_pred_cachepred_add_absorb_clean :
+    forall csmap d a tb bm h,
+      d a = Some tb ->
+      bm h = None ->
+     mem_pred (HighAEQ:= addr_eq_dec) (cachepred csmap bm) (mem_except d a) ✶ a |-> tb =p=>
+     mem_pred (HighAEQ:= addr_eq_dec) (cachepred (Map.add a (h, false) csmap) (upd bm h tb)) d.
+  Proof.
+    intros.
+    eapply pimpl_trans; [ | apply mem_pred_absorb_nop; eauto ].
+    unfold cachepred at 3.
+    rewrite MapFacts.add_eq_o by auto.
+    cancel; eauto.
+    apply mem_pred_pimpl_except; eauto.
+    unfold cachepred; intros.
+    rewrite MapFacts.add_neq_o; eauto.
+    destruct (find a0 csmap) eqn:D; cancel.
+    destruct p_2; cancel;
+    destruct (Nat.eq_dec h p_1); subst; try congruence;
+    rewrite upd_ne; auto.
+    apply upd_eq; auto.
+  Qed.
