src/PermSecInstr.v
@@ -1,125 +1,279 @@
-Require Export PermSec.
+Require Import Pred Mem.
+Require Export PermSec PermHoare PermSepAuto.
 
-
-
-Lemma read_secure:
-  forall s pr a tb,
-    disk s a = Some tb ->
-    permission_secure pr s (Read a) (fun s s' r => s' = blocks_upd s r tb).
-Proof.
-  unfold permission_secure; intros.
-  inv_exec_perm; simpl in *; cleanup.
-  simpl; intuition.
-Qed.
-
-Lemma write_secure:
-  forall pr s a i tb,
-    blocks s i = Some tb ->
-    permission_secure pr s (Write a i) (fun s s' _ => s' = disk_upd s a tb).
-Proof.
-  unfold permission_secure; intros.
-  inv_exec_perm; simpl in *; cleanup.
-  simpl; intuition.
-Qed.
-
-
-Lemma seal_secure:
-  forall pr s t b,
-    can_access pr t ->
-    permission_secure pr s (Seal t b) (fun s s' r => s' = blocks_upd s r (t, b)).
-Proof.
-  unfold permission_secure; intros.
-  inv_exec_perm; simpl in *; cleanup.
-  simpl; intuition.
-Qed.
-
-Lemma unseal_secure:
-  forall pr s i t b,
-    can_access pr t ->
-    blocks s i = Some (t, b) ->
-    permission_secure pr s (Unseal i) (fun s s' r => s' = s /\ r = b).
-Proof.
-  unfold permission_secure; intros.
-  inv_exec_perm; simpl in *; cleanup.
-  simpl; intuition.
-Qed.
-
-Lemma ret_secure:
-  forall T pr s (v: T),
-    permission_secure pr s (Ret v) (fun s s' r => s' = s /\ r = v).
-Proof.
-  unfold permission_secure; intros.
-  inv_exec_perm; simpl in *; cleanup.
-  simpl; intuition.
-Qed.
-
-Lemma run_secure:
-  forall T s (p: prog T) pr pr' post,
-    permission_secure pr' s p post ->
-    permitted pr pr' ->
-    permission_secure pr s (Run pr' p) post.
-Proof.
-  unfold permission_secure; intros.
-  inv_exec_perm; simpl in *.
-  specialize (trace_app H10); intros; cleanup.
-  specialize (H _ _ _ _ H10); intuition.
-  simpl; intuition.
-  eapply trace_secure_permitted; eauto.
-Qed.
 
 Lemma bind_secure:
-  forall T T' (p1: prog T) (p2: T -> prog T') pr s post
-    (post2: state -> state -> T' -> Prop),
-    permission_secure pr s p1 post ->
-    (forall s' s'' tr tr' tr'' r r',
-       exec pr s tr p1 s' (Finished r) tr' ->
-       post s s' r ->
-       exec pr s' tr' (p2 r) s'' (Finished r') tr'' ->
-       post2 s' s'' r' ->
-       post2 s s'' r') ->
-    (forall s' tr tr' r,
-       exec pr s tr p1 s' (Finished r) tr' ->
-       post s s' r ->
-       permission_secure pr s' (p2 r) post2) ->
-    permission_secure pr s (Bind p1 p2) post2.
+  forall T T' (p1: prog T) (p2: T -> prog T') pr d bm,
+    permission_secure d bm pr p1 ->
+    (forall d' bm' tr tr' r,
+       exec pr tr d bm p1 (Finished d' bm' r) tr' ->
+       permission_secure d' bm' pr (p2 r)) ->
+    permission_secure d bm pr (Bind p1 p2).
 Proof.
   unfold permission_secure; intros.
   inv_exec_perm.
+  specialize (trace_app H1); intros; cleanup.
+  specialize (H _ _ _ H1); cleanup.
   specialize (trace_app H2); intros; cleanup.
-  specialize (H _ _ _ _ H2); cleanup.
-  specialize (trace_app H3); intros; cleanup.
-  specialize (H1 _ _ _ _ H2 H4); cleanup.
-  specialize (H1 _ _ _ _ H3); cleanup.
-  intuition.
+  specialize (H0 _ _ _ _ _ H1); cleanup.
+  rewrite <- app_assoc in H2;
+  specialize (H0 _ _ _ H2); cleanup.
   apply trace_secure_app; auto.
-  eauto.
 Qed.
 
-
 Lemma permission_drop_secure:
-  forall s pr1 pr2 T (p: prog T) post,
-    permission_secure pr1 s p post ->
+  forall d bm pr1 pr2 T (p: prog T),
+    permission_secure d bm pr1 p ->
     permitted pr2 pr1 ->
-    (forall s' tr tr2 r, exec pr2 s tr p s' r (tr2++tr) ->
-                      exists tr1, exec pr1 s tr p s' r (tr1++tr) /\ trace_match pr1 pr2 tr1 tr2) ->
-    permission_secure pr2 s p post.
+    (forall tr tr2 r, exec pr2 tr d bm  p r (tr2++tr) ->
+                      exists tr1, exec pr1 tr d bm  p r (tr1++tr) /\ trace_match pr1 pr2 tr1 tr2) ->
+    permission_secure d bm pr2 p.
 Proof.
   unfold permission_secure; intros.
-  specialize (H1 _ _ _ _ H2); cleanup.
-  specialize (H _ _ _ _ H1); intuition.
+  specialize (H1 _ _ _ H2); cleanup.
+  specialize (H _ _ _ H1); intuition.
   eapply trace_secure_match; eauto.
 Qed.
 
-Theorem impl_secure:
-  forall T s (p: prog T) pr
-    (post post': PermProg.state -> PermProg.state -> T -> Prop),
-    permission_secure pr s p post ->
-    (forall s' tr tr' r,
-       exec pr s tr p s' (Finished r) tr' ->
-       post s s' r ->
-       post' s s' r) ->
-    permission_secure pr s p post'.
+
+Lemma read_secure:
+  forall pr a,
+    {< tb F (bm': block_mem),
+       PERM: pr
+       PRE: fun bm =>
+          (F * a|->tb * [[ bm = bm' ]])%pred
+       POST: fun bm =>
+          RET: i
+          (F * a|->tb * [[ bm' i = None ]] *
+          [[ bm = upd (AEQ:= PeanoNat.Nat.eq_dec) bm' i tb ]])%pred
+     >} Read a.
 Proof.
+  unfold corr2; intros.
+  destruct_lift H; cleanup.
+  repeat inv_exec_perm; simpl in *; cleanup.
+  edestruct H3; eauto.
+  pred_apply; cancel.
+  apply ptsto_valid' in H; cleanup; eauto.
+  
+  intuition.
+  eapply bind_secure; intuition.
+  
   unfold permission_secure; intros.
-  specialize (H _ _ _ _ H1); cleanup; eauto.
-Qed. 
+  inv_exec_perm; cleanup; auto.
+  simpl; eauto.
+  
+  unfold permission_secure; intros.
+  clear H1.
+  inv_exec_perm; cleanup; auto.
+  edestruct H3; eauto.
+  pred_apply; cancel; eauto.
+  apply ptsto_valid' in H; cleanup; eauto.
+Qed.
+
+Lemma write_secure:
+  forall pr a i,
+    {< F tb tb' bm',
+       PERM: pr
+       PRE: fun bm =>
+          (F * a|->tb' * [[ bm = bm' ]] * [[ bm i = Some tb ]])%pred
+       POST: fun bm =>
+          RET: tt
+          (F * a|->tb * [[ bm = bm' ]])%pred
+     >} Write a i.
+Proof.
+  unfold corr2; intros.
+   destruct_lift H; cleanup.
+  repeat inv_exec_perm; simpl in *; cleanup.
+  edestruct H3; eauto.
+  admit.
+  intuition eauto.
+  eapply bind_secure; intuition.
+  
+  unfold permission_secure; intros.
+  inv_exec_perm; cleanup; auto.
+  simpl; eauto.
+
+  unfold permission_secure; intros.
+  clear H1.
+  inv_exec_perm; cleanup; auto.
+  edestruct H3; eauto.
+  admit.
+  Unshelve.
+  auto.
+Admitted.
+
+
+Lemma seal_secure:
+  forall pr t b,
+    {< bm',
+       PERM: pr
+       PRE: fun bm =>
+          ([[ can_access pr t ]] * [[ bm = bm' ]])%pred
+       POST: fun bm =>
+          RET : i
+          [[ bm' i = None ]] *
+          [[ bm = upd (AEQ:= PeanoNat.Nat.eq_dec) bm' i (t, b)]]
+     >} Seal t b.
+Proof.
+  unfold corr2; intros.
+  destruct_lift H; cleanup.
+  repeat inv_exec_perm; simpl in *; cleanup.
+  edestruct H3; eauto.
+  pred_apply; cancel.
+
+  intuition eauto.
+  eapply bind_secure; intuition.
+  
+  unfold permission_secure; intros.
+  inv_exec_perm; cleanup; auto.
+  simpl; eauto.
+
+  unfold permission_secure; intros.
+  clear H1.
+  inv_exec_perm; cleanup; auto.
+  edestruct H3; eauto.
+  pred_apply; cancel.
+Qed.
+
+Lemma unseal_secure:
+  forall pr i,
+     {< tb bm',
+       PERM: pr
+       PRE: fun bm =>
+         ([[ can_access pr (fst tb) ]] * [[ bm = bm' ]] * [[ bm i = Some tb ]])%pred
+       POST: fun bm =>
+          RET : b
+          ([[ b = snd tb ]] * [[ bm = bm' ]])%pred
+     >} Unseal i.
+Proof.
+  unfold corr2; intros.
+  destruct_lift H; cleanup.
+  repeat inv_exec_perm; simpl in *; cleanup.
+  edestruct H3; eauto.
+  pred_apply; cancel.
+  intuition eauto.
+  eapply bind_secure; intuition.
+  
+  unfold permission_secure; intros.
+  inv_exec_perm; cleanup; auto.
+  simpl; eauto.
+
+  unfold permission_secure; intros.
+  clear H2.
+  inv_exec_perm; cleanup; auto.
+  edestruct H3; eauto.
+  pred_apply; cancel.
+Qed.
+
+Lemma ret_secure:
+  forall T pr (v: T),
+     {< bm',
+       PERM: pr
+       PRE: fun bm =>
+         [[ bm = bm' ]]
+       POST: fun bm =>
+          RET : r
+          ([[ r = v ]] * [[ bm = bm' ]])
+     >} Ret v.
+Proof.
+  unfold corr2; intros.
+  destruct_lift H; cleanup.
+  repeat inv_exec_perm; simpl in *; cleanup.
+  edestruct H3; eauto.
+  pred_apply; cancel.
+  intuition eauto.
+  eapply bind_secure; intuition.
+  
+  unfold permission_secure; intros.
+  inv_exec_perm; cleanup; auto.
+  simpl; eauto.
+
+  unfold permission_secure; intros.
+  clear H1.
+  inv_exec_perm; cleanup; auto.
+  edestruct H3; eauto.
+  pred_apply; cancel.
+Qed.
+
+Lemma exec_trace_irrelevance:
+  forall T (p: prog T) pr tr tr' tr'' d bm r,
+    exec pr tr d bm p r (tr'++tr) ->
+    exec pr tr'' d bm p r (tr'++tr'').
+Proof.
+  induction p; intros;
+  repeat inv_exec_perm; simpl in *; cleanup;
+  try solve [ econstructor; eauto].
+  specialize (trace_app H8); intros; cleanup.
+  constructor; eauto.
+  specialize (trace_app H0); intros; cleanup.
+  specialize (trace_app H1); intros; cleanup.
+  econstructor; eauto.
+  eapply IHp; eauto.
+  rewrite <- app_assoc in *; eapply H; eauto.
+Qed.
+
+Lemma exec_permission_drop:
+  forall T (p: prog T) pr pr' d bm tr r tr',
+    exec pr' tr d bm p r tr' ->
+    permitted pr pr' ->
+    exists tr'', exec pr tr d bm p r tr''.
+Proof.
+  induction p; intros;
+  repeat inv_exec_perm; simpl in *; cleanup;
+  try solve [ eexists; econstructor; eauto ].
+  specialize (trace_app H0); intros; cleanup.
+  specialize (trace_app H2); intros; cleanup.
+  specialize (IHp _ _ _ _ _ _ _ H0 H1); cleanup.
+  specialize (H _ _ _ _ _ _ _ _ H2 H1); cleanup.
+  specialize (trace_app H3); intros; cleanup.
+  specialize (trace_app H); intros; cleanup.
+  eexists; econstructor; eauto.
+  eapply exec_trace_irrelevance; eauto.
+Qed.
+
+(*
+Lemma exec_trace_match:
+  forall T (p: prog T) pr1 pr2 tr tr1 tr2 d bm r,
+    exec pr2 tr d bm  p r (tr2++tr) ->
+    exec pr1 tr d bm  p r (tr1++tr) ->
+    trace_match pr1 pr2 tr1 tr2.
+Proof.
+  induction p; intros; repeat inv_exec_perm; subst;
+  try solve [ (rewrite H10 in H12
+             || rewrite H7 in H11
+             || rewrite H5 in H8); clear_trace; cleanup; apply trace_match_refl];
+  try solve [ clear_trace; cleanup; apply trace_match_refl].
+  specialize (trace_app H8); intros; cleanup.
+  specialize (trace_app H9); intros; cleanup.
+  simpl; intuition eauto.
+  eapply IHp; eauto.
+  rewrite <- app_assoc; eapply H; eauto.
+Qed.
+*)
+
+
+(* not a right spec *)
+Lemma run_secure:
+  forall E T (p: prog T) pr pr' pre post,
+     {< (e: E),
+       PERM: pr'
+       PRE: fun bm =>
+         pre
+       POST: fun bm =>
+          post
+     >} p ->
+     {< (e:E),
+       PERM: pr
+       PRE: fun bm =>
+         (pre * [[ permitted pr pr']])%pred
+       POST: fun bm =>
+          post
+     >} Run pr' p.
+Proof.
+Abort.
+
+Hint Extern 1 (corr2 _ _ (Bind (Read _) _)) => apply read_secure : prog.
+Hint Extern 1 (corr2 _ _ (Bind (Write _ _) _)) => apply write_secure : prog.
+Hint Extern 1 (corr2 _ _ (Bind (Seal _ _) _)) => apply seal_secure : prog.
+Hint Extern 1 (corr2 _ _ (Bind (Unseal _) _)) => apply unseal_secure : prog.
+Hint Extern 1 (corr2 _ _ (Bind (Ret _) _)) => apply ret_secure : prog.
